Heap/RemoveEdge.v
@@ -5,6 +5,9 @@ Require Import PL.Monad.
 Require Import PL.Monad2.
 Require Import SetsClass.
 Require Import HEAP.Defs.
+Require Import Classical.
+Require Import Coq.Setoids.Setoid.
+Require Import Coq.micromega.Psatz.
 Import SetsNotation
        StateRelMonad
        StateRelMonadOp
@@ -80,8 +83,9 @@ Proof.
     rewrite H.
     rewrite <- H2.
     reflexivity.
-  - apply Hoare_ret'.
+  - unfold Hoare; sets_unfold.
     intros.
+    subst s2.
     tauto.
 Qed.
 
@@ -107,8 +111,9 @@ Proof.
     rewrite H.
     rewrite <- H2.
     reflexivity.
-  - apply Hoare_ret'.
-    intros.
+  - unfold Hoare; sets_unfold.
+  intros.
+  subst s2.
     tauto.
 Qed.
 
@@ -117,14 +122,13 @@ Qed.
 (*********************************************************)
 
 Fact remove_go_left_edge_fact2: forall (v lc: Z),
-  Hoare (fun s => BinaryTree.legal s.(heap) /\ 
-                  BinaryTree.step_l s.(heap) v lc)
+  Hoare (fun s => BinaryTree.legal s.(heap))
         (remove_go_left_edge v lc)
         (fun _ s => BinaryTree.legal s.(heap) /\ 
                     ~ (exists x, BinaryTree.step_l s.(heap) v x) /\ 
                     ~ (exists x, BinaryTree.step_u s.(heap) lc x)).
-Proof.
-  intros.
+(* Proof. *)
+  (* intros.
   unfold remove_go_left_edge, Hoare; sets_unfold.
   intros.
   destruct H as [? Hx].
@@ -318,8 +322,19 @@ Proof.
       - rewrite <- H10; tauto.
       - rewrite <- H11; tauto. 
     }
-    destruct H.
+    destruct H. *)
+Proof.
+  unfold Hoare, remove_go_left_edge; sets_unfold.
+  intros.
+  destruct H0 as [? [? [? [? [? [? ?]]]]]].
+  unfold BinaryTree.step_l.
+  unfold not.
+  split.
+  - intros.
+    split.
+    
 Admitted.
+
 
 Fact remove_go_right_edge_fact2: forall (v rc: Z),
   Hoare (fun s => BinaryTree.legal s.(heap))
@@ -354,6 +369,11 @@ Fact remove_go_right_edge'_fact2:
                       | by_exist rc => ~ (exists x, BinaryTree.step_u s.(heap) rc x)
                       | by_empty => True
                       end).
+Proof.
+  intros.
+  unfold remove_go_right_edge'.
+  destruct a.
+  - apply remove_go_right_edge_fact2.
 Admitted.
 
 (*********************************************************)
@@ -364,42 +384,182 @@ Fact remove_go_left_edge_fact3_l:
     Hoare (fun s => ~ exists x, BinaryTree.step_l s.(heap) u x)
           (remove_go_left_edge v a)
           (fun _ s => ~ exists x, BinaryTree.step_l s.(heap) u x).
-Admitted.
+Proof.
+  unfold Hoare, remove_go_left_edge; sets_unfold.
+  intros.
+  destruct H0 as [? [? [? [? [? [? ?]]]]]].
+  unfold BinaryTree.step_l.
+  unfold not.
+  intros.
+  destruct H6.
+  destruct H6 as [e0 ?].
+  pose proof (classic (e0 = x)).
+  destruct H7.
+  + subst e0.
+    destruct H6. destruct H6.
+     tauto.
+  + pose proof H5 e0 H7.
+    unfold BinaryTree.step_l in H.
+  assert (exists x e : Z, BinaryTree.step_aux s1.(heap) e u x /\ (s1.(heap)).(go_left) e).
+  * exists x0, e0.
+    pose proof H8 u x0.
+    destruct H6.
+    destruct H9.
+    rewrite <- H11.
+    tauto.
+  *tauto.
+Qed.
 
 Fact remove_go_left_edge_fact3_r:
   forall (v: Z) (a: Z) (u: Z),
     Hoare (fun s => ~ exists x, BinaryTree.step_r s.(heap) u x)
           (remove_go_left_edge v a)
           (fun _ s => ~ exists x, BinaryTree.step_r s.(heap) u x).
-Admitted.
+Proof.
+  unfold Hoare, remove_go_left_edge; sets_unfold.
+  intros.
+  destruct H0 as [? [? [? [? [? [? ?]]]]]].
+  unfold BinaryTree.step_r.
+  unfold not.
+  intros.
+  destruct H6.
+  destruct H6 as [e0 ?].
+  pose proof (classic (e0 = x)).
+  destruct H7.
+  + subst e0.
+    destruct H6. destruct H6.
+     tauto.
+  + pose proof H5 e0 H7.
+    unfold BinaryTree.step_r in H.
+  assert (exists x e : Z, BinaryTree.step_aux s1.(heap) e u x /\ (s1.(heap)).(go_right) e).
+  * exists x0, e0.
+    pose proof H8 u x0.
+    destruct H6.
+    destruct H9.
+    unfold BinaryTree.go_right.
+    unfold BinaryTree.go_right in H10.
+    rewrite <- H11.
+    tauto.
+  *tauto.
+Qed.
 
 Fact remove_go_left_edge_fact3_u:
   forall (v: Z) (a: Z) (u: Z),
     Hoare (fun s => ~ exists x, BinaryTree.step_u s.(heap) u x)
           (remove_go_left_edge v a)
           (fun _ s => ~ exists x, BinaryTree.step_u s.(heap) u x).
-Admitted.
+Proof.
+  unfold Hoare, remove_go_left_edge; sets_unfold.
+  intros.
+  destruct H0 as [? [? [? [? [? [? ?]]]]]].
+  unfold BinaryTree.step_u.
+  unfold not.
+  intros.
+  destruct H6.
+  destruct H6 as [e0 ?].
+  pose proof (classic (e0 = x)).
+  destruct H7.
+  + subst e0.
+    destruct H6.
+     tauto.
+  + pose proof H5 e0 H7.
+    unfold BinaryTree.step_u in H.
+  assert (exists x e : Z, BinaryTree.step_aux s1.(heap) e x u).
+  * exists x0, e0.
+    pose proof H8 x0 u.
+    tauto.
+  *tauto.
+Qed.
 
 Fact remove_go_right_edge_fact3_l:
   forall (v: Z) (a: Z) (u: Z),
     Hoare (fun s => ~ exists x, BinaryTree.step_l s.(heap) u x)
           (remove_go_right_edge v a)
           (fun _ s => ~ exists x, BinaryTree.step_l s.(heap) u x).
+Proof.
+  unfold Hoare, remove_go_right_edge; sets_unfold.
+  intros.
+  destruct H0 as [? [? [? [? [? [? ?]]]]]].
+  unfold BinaryTree.step_l.
+  unfold not.
+  intros.
+  destruct H6.
+  destruct H6 as [e0 ?].
+  pose proof (classic (e0 = x)).
+  destruct H7.
+  + subst e0.
+    destruct H6. destruct H6.
+    tauto.
+  + pose proof H5 e0 H7.
+    unfold BinaryTree.step_l in H.
+  assert (exists x e : Z, BinaryTree.step_aux s1.(heap) e u x /\ (s1.(heap)).(go_left) e).
+  * exists x0, e0.
+    pose proof H8 u x0.
+    destruct H6.
+    destruct H9.    
+    unfold BinaryTree.go_right in H11.
 Admitted.
 
-Fact remove_go_right_edge_fact3_r:
+
+Fact remove_go_right_edge_fact3_r: 
   forall (v: Z) (a: Z) (u: Z),
     Hoare (fun s => ~ exists x, BinaryTree.step_r s.(heap) u x)
           (remove_go_right_edge v a)
           (fun _ s => ~ exists x, BinaryTree.step_r s.(heap) u x).
-Admitted.
+Proof.
+unfold Hoare, remove_go_left_edge; sets_unfold.
+intros.
+destruct H0 as [? [? [? [? [? [? ?]]]]]].
+unfold BinaryTree.step_l.
+unfold not.
+intros.
+destruct H6.
+destruct H6 as [e0 ?].
+pose proof (classic (e0 = x)).
+destruct H7.
++ subst e0.
+  destruct H6. destruct H6.
+   tauto.
++ pose proof H5 e0 H7.
+  unfold BinaryTree.step_l in H.
+assert (exists x e : Z, BinaryTree.step_aux s1.(heap) e u x /\ (s1.(heap)).(go_right) e).
+* exists x0, e0.
+  pose proof H8 u x0.
+  destruct H6.
+  destruct H9.
+  rewrite <- H11.
+  tauto.
+*tauto.
+Qed.
+  
 
 Fact remove_go_right_edge_fact3_u:
   forall (v: Z) (a: Z) (u: Z),
     Hoare (fun s => ~ exists x, BinaryTree.step_u s.(heap) u x)
           (remove_go_right_edge v a)
           (fun _ s => ~ exists x, BinaryTree.step_u s.(heap) u x).
-Admitted.
+Proof.
+  unfold Hoare, remove_go_right_edge; sets_unfold.
+  intros.
+  destruct H0 as [? [? [? [? [? [? ?]]]]]].
+  unfold BinaryTree.step_u.
+  unfold not.
+  intros.
+  destruct H6.
+  destruct H6 as [e0 ?].
+  pose proof (classic (e0 = x)).
+  destruct H7.
+  + subst e0.
+    destruct H6.
+     tauto.
+  + pose proof H5 e0 H7.
+    unfold BinaryTree.step_u in H.
+  assert (exists x e : Z, BinaryTree.step_aux s1.(heap) e x u).
+  * exists x0, e0.
+    pose proof H8 x0 u.
+    tauto.
+  *tauto.
+Qed.
 
 (*********************************************************)
 (*********************************************************)
@@ -409,42 +569,103 @@ Fact remove_go_left_edge'_fact3_l:
     Hoare (fun s => ~ exists x, BinaryTree.step_l s.(heap) u x)
           (remove_go_left_edge' v a)
           (fun _ s => ~ exists x, BinaryTree.step_l s.(heap) u x).
-Admitted.
+Proof.
+  intros.
+  destruct a.
+  - simpl.
+    apply remove_go_left_edge_fact3_l.
+  - simpl.
+    unfold Hoare; sets_unfold.
+    intros.
+    subst s2.
+    tauto.
+Qed.
+
 
 Fact remove_go_left_edge'_fact3_r:
   forall (v: Z) (a: ExistOrEmpty) (u: Z),
     Hoare (fun s => ~ exists x, BinaryTree.step_r s.(heap) u x)
           (remove_go_left_edge' v a)
           (fun _ s => ~ exists x, BinaryTree.step_r s.(heap) u x).
-Admitted.
+Proof.
+  intros.
+  destruct a.
+  - simpl.
+    apply remove_go_left_edge_fact3_r.
+  - simpl.
+    unfold Hoare; sets_unfold.
+    intros.
+    subst s2.
+    tauto.
+Qed.
 
 Fact remove_go_left_edge'_fact3_u:
   forall (v: Z) (a: ExistOrEmpty) (u: Z),
     Hoare (fun s => ~ exists x, BinaryTree.step_u s.(heap) u x)
           (remove_go_left_edge' v a)
           (fun _ s => ~ exists x, BinaryTree.step_u s.(heap) u x).
-Admitted.
+Proof.
+  intros.
+  destruct a.
+  - simpl.
+    apply remove_go_left_edge_fact3_u.
+  - simpl.
+    unfold Hoare; sets_unfold.
+    intros.
+    subst s2.
+    tauto.
+Qed.
 
 Fact remove_go_right_edge'_fact3_l:
   forall (v: Z) (a: ExistOrEmpty) (u: Z),
     Hoare (fun s => ~ exists x, BinaryTree.step_l s.(heap) u x)
           (remove_go_right_edge' v a)
           (fun _ s => ~ exists x, BinaryTree.step_l s.(heap) u x).
-Admitted.
+Proof.
+  intros.
+  destruct a.
+  - simpl.
+    apply remove_go_right_edge_fact3_l.
+  - simpl.
+    unfold Hoare; sets_unfold.
+    intros.
+    subst s2.
+    tauto.
+Qed.
 
 Fact remove_go_right_edge'_fact3_r:
   forall (v: Z) (a: ExistOrEmpty) (u: Z),
     Hoare (fun s => ~ exists x, BinaryTree.step_r s.(heap) u x)
           (remove_go_right_edge' v a)
           (fun _ s => ~ exists x, BinaryTree.step_r s.(heap) u x).
-Admitted.
+Proof.
+  intros.
+  destruct a.
+  - simpl.
+    apply remove_go_right_edge_fact3_r.
+  - simpl.
+    unfold Hoare; sets_unfold.
+    intros.
+    subst s2.
+    tauto.
+Qed.
 
 Fact remove_go_right_edge'_fact3_u:
   forall (v: Z) (a: ExistOrEmpty) (u: Z),
     Hoare (fun s => ~ exists x, BinaryTree.step_u s.(heap) u x)
           (remove_go_right_edge' v a)
           (fun _ s => ~ exists x, BinaryTree.step_u s.(heap) u x).
-Admitted.
+Proof.
+  intros.
+  destruct a.
+  - simpl.
+    apply remove_go_right_edge_fact3_u.
+  - simpl.
+    unfold Hoare; sets_unfold.
+    intros.
+    subst s2.
+    tauto.
+Qed.
 
 (*********************************************************)
 (*********************************************************)
@@ -460,7 +681,35 @@ Fact remove_go_left_edge_fact4_l:
                       | by_exist lc => ~ (exists x : Z, BinaryTree.step_l s.(heap) lc x)
                       | by_empty => True
                       end).
-Admitted.
+Proof.
+  intros.
+  unfold Hoare, remove_go_left_edge; sets_unfold.
+  intros.
+  destruct H0 as [? [? [? [? [? [? ?]]]]]].
+  destruct u.
+  2 : { tauto. }
+  unfold BinaryTree.step_l.
+  unfold not.
+  intros.
+  destruct H6.
+  destruct H6 as [e0 ?].
+  pose proof (classic (e0 = x)).
+  destruct H7.
+  + subst e0.
+    destruct H6. destruct H6.
+    tauto.
+  + pose proof H5 e0 H7.
+    unfold BinaryTree.step_l in H.
+  assert (exists x e : Z, BinaryTree.step_aux s1.(heap) e a1 x /\ (s1.(heap)).(go_left) e).
+  * exists x0, e0.
+    pose proof H8 a1 x0.
+    destruct H6.
+    destruct H9.
+    rewrite <- H11.
+    tauto.
+  *tauto.
+Qed.
+  
 
 Fact remove_go_left_edge_fact4_r:
   forall (v: Z) (a: Z) (u: ExistOrEmpty),
@@ -473,7 +722,36 @@ Fact remove_go_left_edge_fact4_r:
                       | by_exist lc => ~ (exists x : Z, BinaryTree.step_r s.(heap) lc x)
                       | by_empty => True
                       end).
-Admitted.
+Proof.
+  intros.
+  unfold Hoare, remove_go_left_edge; sets_unfold.
+  intros.
+  destruct H0 as [? [? [? [? [? [? ?]]]]]].
+  destruct u.
+  2 : { tauto. }
+  unfold BinaryTree.step_r.
+  unfold not.
+  intros.
+  destruct H6.
+  destruct H6 as [e0 ?].
+  pose proof (classic (e0 = x)).
+  destruct H7.
+  + subst e0.
+    destruct H6. destruct H6.
+    tauto.
+  + pose proof H5 e0 H7.
+    unfold BinaryTree.step_r in H.
+  assert (exists x e : Z, BinaryTree.step_aux s1.(heap) e a1 x /\ (s1.(heap)).(go_right) e).
+  * exists x0, e0.
+    pose proof H8 a1 x0.
+    destruct H6.
+    destruct H9.
+    unfold BinaryTree.go_right in H11.
+    unfold BinaryTree.go_right.
+    rewrite <- H11.
+    tauto.
+  *tauto.
+Qed.
 
 Fact remove_go_left_edge_fact4_u:
   forall (v: Z) (a: Z) (u: ExistOrEmpty),
@@ -486,7 +764,31 @@ Fact remove_go_left_edge_fact4_u:
                       | by_exist lc => ~ (exists x : Z, BinaryTree.step_u s.(heap) lc x)
                       | by_empty => True
                       end).
-Admitted.
+Proof.
+  intros.
+  unfold Hoare, remove_go_left_edge; sets_unfold.
+  intros.
+  destruct H0 as [? [? [? [? [? [? ?]]]]]].
+  destruct u.
+  2 : { tauto. }
+  unfold BinaryTree.step_u.
+  unfold not.
+  intros.
+  destruct H6.
+  destruct H6 as [e0 ?].
+  pose proof (classic (e0 = x)).
+  destruct H7.
+  + subst e0.
+    destruct H6.
+    tauto.
+  + pose proof H5 e0 H7.
+    unfold BinaryTree.step_u in H.
+  assert (exists x e : Z, BinaryTree.step_aux s1.(heap) e x a1).
+  * exists x0, e0.
+    pose proof H8 x0 a1.
+    tauto.
+  *tauto.
+Qed.
 
 Fact remove_go_right_edge_fact4_l:
   forall (v: Z) (a: Z) (u: ExistOrEmpty),
@@ -512,7 +814,36 @@ Fact remove_go_right_edge_fact4_r:
                       | by_exist lc => ~ (exists x : Z, BinaryTree.step_r s.(heap) lc x)
                       | by_empty => True
                       end).
-Admitted.
+Proof.
+  intros.
+  unfold Hoare, remove_go_right_edge; sets_unfold.
+  intros.
+  destruct H0 as [? [? [? [? [? [? ?]]]]]].
+  destruct u.
+  2 : { tauto. }
+  unfold BinaryTree.step_r.
+  unfold not.
+  intros.
+  destruct H6.
+  destruct H6 as [e0 ?].
+  pose proof (classic (e0 = x)).
+  destruct H7.
+  + subst e0.
+    destruct H6. destruct H6.
+    tauto.
+  + pose proof H5 e0 H7.
+    unfold BinaryTree.step_r in H.
+  assert (exists x e : Z, BinaryTree.step_aux s1.(heap) e a1 x /\ (s1.(heap)).(go_right) e).
+  * exists x0, e0.
+    pose proof H8 a1 x0.
+    destruct H6.
+    destruct H9.
+    unfold BinaryTree.go_right in H11.
+    unfold BinaryTree.go_right.
+    rewrite <- H11.
+    tauto.
+  *tauto.
+Qed.
 
 Fact remove_go_right_edge_fact4_u:
   forall (v: Z) (a: Z) (u: ExistOrEmpty),
@@ -525,8 +856,31 @@ Fact remove_go_right_edge_fact4_u:
                       | by_exist lc => ~ (exists x : Z, BinaryTree.step_u s.(heap) lc x)
                       | by_empty => True
                       end).
-Admitted.
-
+Proof.
+  intros.
+  unfold Hoare, remove_go_right_edge; sets_unfold.
+  intros.
+  destruct H0 as [? [? [? [? [? [? ?]]]]]].
+  destruct u.
+  2 : { tauto. }
+  unfold BinaryTree.step_u.
+  unfold not.
+  intros.
+  destruct H6.
+  destruct H6 as [e0 ?].
+  pose proof (classic (e0 = x)).
+  destruct H7.
+  + subst e0.
+    destruct H6.
+    tauto.
+  + pose proof H5 e0 H7.
+    unfold BinaryTree.step_u in H.
+  assert (exists x e : Z, BinaryTree.step_aux s1.(heap) e x a1).
+  * exists x0, e0.
+    pose proof H8 x0 a1.
+    tauto.
+  *tauto.
+Qed.
 
 (*********************************************************)
 (*********************************************************)
@@ -542,7 +896,16 @@ Fact remove_go_left_edge'_fact4_l:
                       | by_exist lc => ~ (exists x : Z, BinaryTree.step_l s.(heap) lc x)
                       | by_empty => True
                       end).
-Admitted.
+Proof.
+  intros.
+  unfold remove_go_left_edge'.
+  induction a.
+  - apply remove_go_left_edge_fact4_l.
+  - unfold Hoare; sets_unfold.
+    intros.
+    subst s2.
+    tauto.
+Qed.
 
 Fact remove_go_left_edge'_fact4_r:
   forall (v: Z) (a: ExistOrEmpty) (u: ExistOrEmpty),
@@ -555,7 +918,16 @@ Fact remove_go_left_edge'_fact4_r:
                       | by_exist lc => ~ (exists x : Z, BinaryTree.step_r s.(heap) lc x)
                       | by_empty => True
                       end).
-Admitted.
+Proof.
+  intros.
+  unfold remove_go_left_edge'.
+  induction a.
+  - apply remove_go_left_edge_fact4_r.
+  - unfold Hoare; sets_unfold.
+    intros.
+    subst s2.
+    tauto.
+Qed.
 
 Fact remove_go_left_edge'_fact4_u:
   forall (v: Z) (a: ExistOrEmpty) (u: ExistOrEmpty),
@@ -568,7 +940,16 @@ Fact remove_go_left_edge'_fact4_u:
                       | by_exist lc => ~ (exists x : Z, BinaryTree.step_u s.(heap) lc x)
                       | by_empty => True
                       end).
-Admitted.
+Proof.
+  intros.
+  unfold remove_go_left_edge'.
+  induction a.
+  - apply remove_go_left_edge_fact4_u.
+  - unfold Hoare; sets_unfold.
+    intros.
+    subst s2.
+    tauto.
+Qed.
 
 Fact remove_go_right_edge'_fact4_l:
   forall (v: Z) (a: ExistOrEmpty) (u: ExistOrEmpty),
@@ -581,7 +962,16 @@ Fact remove_go_right_edge'_fact4_l:
                       | by_exist lc => ~ (exists x : Z, BinaryTree.step_l s.(heap) lc x)
                       | by_empty => True
                       end).
-Admitted.
+Proof.
+  intros.
+  unfold remove_go_right_edge'.
+  induction a.
+  - apply remove_go_right_edge_fact4_l.
+  - unfold Hoare; sets_unfold.
+    intros.
+    subst s2.
+    tauto.
+Qed.
 
 Fact remove_go_right_edge'_fact4_r:
   forall (v: Z) (a: ExistOrEmpty) (u: ExistOrEmpty),
@@ -594,7 +984,16 @@ Fact remove_go_right_edge'_fact4_r:
                       | by_exist lc => ~ (exists x : Z, BinaryTree.step_r s.(heap) lc x)
                       | by_empty => True
                       end).
-Admitted.
+Proof.
+  intros.
+  unfold remove_go_right_edge'.
+  induction a.
+  - apply remove_go_right_edge_fact4_r.
+  - unfold Hoare; sets_unfold.
+    intros.
+    subst s2.
+    tauto.
+Qed.
 
 Fact remove_go_right_edge'_fact4_u:
   forall (v: Z) (a: ExistOrEmpty) (u: ExistOrEmpty),
@@ -607,10 +1006,17 @@ Fact remove_go_right_edge'_fact4_u:
                       | by_exist lc => ~ (exists x : Z, BinaryTree.step_u s.(heap) lc x)
                       | by_empty => True
                       end).
-Admitted.
-
+Proof.
+  intros.
+  unfold remove_go_right_edge'.
+  induction a.
+  - apply remove_go_right_edge_fact4_u.
+  - unfold Hoare; sets_unfold.
+    intros.
+    subst s2.
+    tauto.
+Qed.
 
 (*********************************************************)
 (*********************************************************)
-
 
