Heap/Swapvu.v
@@ -10,6 +10,9 @@ Require Import Coq.Setoids.Setoid.
 Require Import Coq.micromega.Psatz.
 Require Import HEAP.AddEdge.
 Require Import HEAP.RemoveEdge.
+Require Import Classical.
+Require Import Coq.Setoids.Setoid.
+Require Import Coq.micromega.Psatz.
 Import SetsNotation
        StateRelMonad
        StateRelMonadOp
@@ -31,6 +34,13 @@ Proof.
   - rewrite H1. tauto.
 Qed.
 
+Fact get_fa'_fact: forall (fa: Z) P, 
+  Hoare P (get_fa' fa) 
+    (fun a s => P s /\ match a with
+                      | by_exist gf => BinaryTree.step_u s.(heap) fa gf
+                      | by_empty => ~ (exists x, BinaryTree.step_u s.(heap) fa x)
+                      end). 
+Admitted.
 
 Fact get_lc_fact: forall (v: Z) P, 
   Hoare P (get_lc v) (fun lc s => P s /\ BinaryTree.step_l s.(heap) v lc).
@@ -62,6 +72,9 @@ Proof.
     tauto.
 Qed.
 
+Fact get_rc_fact: forall (v: Z) P, 
+  Hoare P (get_rc v) (fun rc s => P s /\ BinaryTree.step_r s.(heap) v rc).
+Admitted.
 
 Fact get_rc'_fact: forall (v: Z) P, 
   Hoare P (get_rc' v)
@@ -73,11 +86,21 @@ Admitted.
 
 Fact get_dir_fact: forall (fa v: Z) P, 
   Hoare P (get_dir fa v)
-    (fun dir s => P s /\
-      (
-        (dir = 0 /\ BinaryTree.step_l s.(heap) fa v) \/
-        (dir = 1 /\ BinaryTree.step_r s.(heap) fa v))
-      ).
+    (fun dir s => P s /\ (dir = 0 \/ dir = 1) /\
+                  ((dir = 0 /\ BinaryTree.step_l s.(heap) fa v) \/
+                   (dir = 1 /\ BinaryTree.step_r s.(heap) fa v))).
+Admitted.
+
+Fact get_dir'_fact:
+  forall (fa: ExistOrEmpty) (v: Z) P,
+    Hoare P (get_dir' fa v)
+      (fun dir s => P s /\
+        (
+          match fa with
+          | by_exist fa => (dir = 0 /\ BinaryTree.step_l s.(heap) fa v) \/
+                           (dir = 1 /\ BinaryTree.step_r s.(heap) fa v)
+          | by_empty => ~ (exists x, BinaryTree.step_u s.(heap) v x)
+          end)).
 Admitted.
 
 Fact swap_v_fa_fact1: forall (v fa: Z) (V: Z -> Prop), 
@@ -115,6 +138,123 @@ Fact swap_v_fa_fact3: forall (v fa: Z) (V: Z -> Prop),
     (fun _ s => Abs s.(heap) V).
 Admitted.
 
+
+Lemma L1: forall (v fa: Z) (lc_v rc_v lc_fa rc_fa gf: ExistOrEmpty)
+  (dir_fa_v: Z) (s: state), 
+    ((((((BinaryTree.legal s.(heap) /\ BinaryTree.step_u s.(heap) v fa) /\
+    match lc_v with
+    | by_exist lc => BinaryTree.step_l s.(heap) v lc
+    | by_empty => ~ (exists x : Z, BinaryTree.step_l s.(heap) v x)
+    end) /\
+    match rc_v with
+    | by_exist rc => BinaryTree.step_r s.(heap) v rc
+    | by_empty => ~ (exists x : Z, BinaryTree.step_r s.(heap) v x)
+    end) /\
+    match lc_fa with
+    | by_exist lc => BinaryTree.step_l s.(heap) fa lc
+    | by_empty => ~ (exists x : Z, BinaryTree.step_l s.(heap) fa x)
+    end) /\
+    match rc_fa with
+    | by_exist rc => BinaryTree.step_r s.(heap) fa rc
+    | by_empty => ~ (exists x : Z, BinaryTree.step_r s.(heap) fa x)
+    end) /\
+    match gf with
+    | by_exist gf0 => BinaryTree.step_u s.(heap) fa gf0
+    | by_empty => ~ (exists x : Z, BinaryTree.step_u s.(heap) fa x)
+    end) /\
+    (dir_fa_v = 0 \/ dir_fa_v = 1) /\
+    (dir_fa_v = 0 /\ BinaryTree.step_l s.(heap) fa v \/
+     dir_fa_v = 1 /\ BinaryTree.step_r s.(heap) fa v)
+    -> 
+      ((((((BinaryTree.legal s.(heap) /\ BinaryTree.step_u s.(heap) v fa) /\
+      match lc_v with
+      | by_exist lc => BinaryTree.step_l s.(heap) v lc
+      | by_empty => ~ (exists x : Z, BinaryTree.step_l s.(heap) v x)
+      end)
+      /\
+      match rc_v with
+      | by_exist rc => BinaryTree.step_r s.(heap) v rc
+      | by_empty => ~ (exists x : Z, BinaryTree.step_r s.(heap) v x)
+      end)
+      /\
+      match lc_fa with
+      | by_exist lc => BinaryTree.step_l s.(heap) fa lc
+      | by_empty => ~ (exists x : Z, BinaryTree.step_l s.(heap) fa x)
+      end)
+      /\
+      match rc_fa with
+      | by_exist rc => BinaryTree.step_r s.(heap) fa rc
+      | by_empty => ~ (exists x : Z, BinaryTree.step_r s.(heap) fa x)
+      end)
+      /\
+      (gf = by_empty -> ~ (exists x : Z, BinaryTree.step_u s.(heap) fa x)))
+      /\ 
+      (dir_fa_v = 0 \/ dir_fa_v = 1)
+      /\
+      (dir_fa_v = 0 -> lc_fa = by_exist v)
+      /\ 
+      (dir_fa_v = 1 -> rc_fa = by_exist v)
+      /\ 
+      ~ fa = v
+      /\ 
+      ~ v = fa
+      /\ 
+      ~ lc_v = rc_v 
+      /\ 
+      ~ lc_fa = rc_fa
+      /\ 
+      match gf with 
+      | by_exist fa_fa => ~ v = fa_fa 
+      | by_empty => True
+      end
+      /\ 
+      match gf with 
+      | by_exist fa_fa => ~ fa = fa_fa 
+      | by_empty => True
+      end
+      /\ 
+      match lc_v with
+      | by_exist lc_v => lc_v <> v 
+      | by_empty => True
+      end
+      /\ 
+      match lc_v with
+      | by_exist lc_v => lc_v <> fa 
+      | by_empty => True
+      end
+      /\ 
+      match lc_v with
+      | by_exist lc_v => fa <> lc_v 
+      | by_empty => True
+      end
+      /\ 
+      match rc_v with
+      | by_exist rc_v => rc_v <> fa
+      | by_empty => True
+      end
+      /\ 
+      match rc_v with
+      | by_exist rc_v => fa <> rc_v
+      | by_empty => True
+      end
+      /\ 
+      match rc_v with
+      | by_exist rc_v => rc_v <> v
+      | by_empty => True
+      end
+      /\ 
+      match lc_v, rc_v with
+      | by_exist lc_v, by_exist rc_v => ~ lc_v = rc_v
+      | by_empty, _ => True
+      | _, by_empty => True
+      end
+      /\ 
+      match rc_fa with
+      | by_exist rc_fa => rc_fa <> fa
+      | by_empty => True
+      end.
+Admitted.
+
 Fact swap_v_fa_fact4: forall (v fa: Z), 
   Hoare
     (fun s => BinaryTree.legal s.(heap) /\
@@ -128,14 +268,37 @@ Proof.
   eapply Hoare_bind; [apply get_rc'_fact| cbv beta; intros rc_v].
   eapply Hoare_bind; [apply get_lc'_fact| cbv beta; intros lc_fa].
   eapply Hoare_bind; [apply get_rc'_fact| cbv beta; intros rc_fa].
+  eapply Hoare_bind; [apply get_fa'_fact| cbv beta; intros gf].
   eapply Hoare_bind; [apply get_dir_fact| cbv beta; intros dir_fa_v].
+  eapply Hoare_conseq_pre; [apply L1| ].
+  eapply Hoare_irr_right.
+  intros.
   eapply Hoare_bind.
-  { eapply Hoare_conseq_pre.
-    2: { apply remove_go_left_edge'_fact2. }
-    + tauto. }
+  { eapply Hoare_conj.
+    + eapply Hoare_conseq_pre.
+      2: { apply remove_go_left_edge'_fact2. }
+      tauto.
+    + assert (Hoare
+                (fun s => BinaryTree.legal s.(heap) /\
+                  (gf = by_empty -> ~ (exists x : Z, BinaryTree.step_u s.(heap) fa x)))
+                (remove_go_left_edge' v lc_v) 
+                (fun _ s => (gf = by_empty -> ~ (exists x : Z, BinaryTree.step_u s.(heap) fa x)))).
+      {
+        pose proof remove_go_left_edge'_fact3_u v lc_v fa.
+        revert H0.
+        unfold Hoare; sets_unfold; intros.
+        destruct H1.
+        pose proof H4 H3.
+        pose proof H0 _ _ _ H5 H2.
+        tauto.
+      }
+      eapply Hoare_conseq_pre.
+      2: { apply H0. }
+      tauto.
+  }
   cbv beta; intros _.
   eapply Hoare_bind.
-  { eapply Hoare_conj3.
+  { eapply Hoare_conj4.
     + eapply Hoare_conseq_pre.
       2: { apply remove_go_right_edge'_fact2. }
       tauto.
@@ -145,10 +308,27 @@ Proof.
     + eapply Hoare_conseq_pre.
       2: { apply (remove_go_right_edge'_fact4_u _ _ lc_v). }
       tauto.
+    + assert (Hoare
+                (fun s => BinaryTree.legal s.(heap) /\
+                  (gf = by_empty -> ~ (exists x : Z, BinaryTree.step_u s.(heap) fa x)))
+                (remove_go_right_edge' v rc_v) 
+                (fun _ s => (gf = by_empty -> ~ (exists x : Z, BinaryTree.step_u s.(heap) fa x)))).
+      {
+        pose proof remove_go_right_edge'_fact3_u v rc_v fa.
+        revert H0.
+        unfold Hoare; sets_unfold; intros.
+        destruct H1.
+        pose proof H4 H3.
+        pose proof H0 _ _ _ H5 H2.
+        tauto.
+      }
+      eapply Hoare_conseq_pre.
+      2: { apply H0. }
+      tauto.
   }
   cbv beta; intros _.
   eapply Hoare_bind.
-  { eapply Hoare_conj5.
+  { eapply Hoare_conj6.
     + eapply Hoare_conseq_pre.
       2: { apply remove_go_left_edge'_fact2. }
       tauto.
@@ -164,10 +344,27 @@ Proof.
     + eapply Hoare_conseq_pre.
       2: { apply (remove_go_left_edge'_fact4_u _ _ rc_v). }
       tauto.
+    + assert (Hoare
+                (fun s => BinaryTree.legal s.(heap) /\
+                  (gf = by_empty -> ~ (exists x : Z, BinaryTree.step_u s.(heap) fa x)))
+                (remove_go_left_edge' fa lc_fa) 
+                (fun _ s => (gf = by_empty -> ~ (exists x : Z, BinaryTree.step_u s.(heap) fa x)))).
+      {
+        pose proof remove_go_left_edge'_fact3_u fa lc_fa fa.
+        revert H0.
+        unfold Hoare; sets_unfold; intros.
+        destruct H1.
+        pose proof H4 H3.
+        pose proof H0 _ _ _ H5 H2.
+        tauto.
+      }
+      eapply Hoare_conseq_pre.
+      2: { apply H0. }
+      tauto.
   }
   cbv beta; intros _.
   eapply Hoare_bind.
-  { eapply Hoare_conj7.
+  { eapply Hoare_conj8.
     + eapply Hoare_conseq_pre.
       2: { apply remove_go_right_edge'_fact2. }
       tauto.
@@ -189,14 +386,29 @@ Proof.
     + eapply Hoare_conseq_pre.
       2: { apply (remove_go_right_edge'_fact4_u _ _ lc_fa). }
       tauto.
+    + assert (Hoare
+                (fun s => BinaryTree.legal s.(heap) /\
+                  (gf = by_empty -> ~ (exists x : Z, BinaryTree.step_u s.(heap) fa x)))
+                (remove_go_right_edge' fa rc_fa) 
+                (fun _ s => (gf = by_empty -> ~ (exists x : Z, BinaryTree.step_u s.(heap) fa x)))).
+      {
+        pose proof remove_go_right_edge'_fact3_u fa rc_fa fa.
+        revert H0.
+        unfold Hoare; sets_unfold; intros.
+        destruct H1.
+        pose proof H4 H3.
+        pose proof H0 _ _ _ H5 H2.
+        tauto.
+      }
+      eapply Hoare_conseq_pre.
+      2: { apply H0. }
+      tauto.
   }
   cbv beta; intros _.
   eapply Hoare_bind.
-  { eapply Hoare_choice.
-    2: {
-      eapply Hoare_bind; [apply get_fa_fact| cbv beta; intros gf].
-      eapply Hoare_choice.
-      * apply Hoare_test_bind.
+  { destruct gf.
+    * eapply Hoare_choice.
+      - apply Hoare_test_bind.
         eapply Hoare_bind.
         { 
           eapply Hoare_conj9.
@@ -226,52 +438,199 @@ Proof.
             tauto.
           + eapply Hoare_conseq_pre.
             2: { apply (remove_go_left_edge_fact4_u _ _ rc_fa). }
-            tauto.
+            tauto.  
         }
         cbv beta; intros _.
-        eapply Hoare_conj9.
+        eapply Hoare_conj10.
         + eapply Hoare_conseq_pre.
           2: { apply add_go_left_edge_fact2. }
-          admit.
+          intros.
+          destruct H0 as [H1 [_ [_ [_ [_ [H2 H3]]]]]].
+          destruct H as [H4 [H5 [H6 _]]].
+          pose proof (classic(dir_fa_v = 0)).
+          destruct H.
+          ++ pose proof H5 H.
+             subst lc_fa.
+             tauto.
+          ++ destruct H4.
+             -- tauto.
+             -- pose proof H6 H0.
+                subst rc_fa.
+                tauto.
         + eapply Hoare_conseq_pre.
           2: { apply (add_go_left_edge_fact3_l _ _ v). }
-          admit.
+          simpl; tauto.
         + eapply Hoare_conseq_pre.
           2: { apply (add_go_left_edge_fact3_r _ _ v). }
-          admit.
+          simpl; tauto.
         + eapply Hoare_conseq_pre.
           2: { apply (add_go_left_edge_fact4_u _ _ lc_v). }
-          admit.
+          simpl. destruct lc_v; tauto.
         + eapply Hoare_conseq_pre.
           2: { apply (add_go_left_edge_fact4_u _ _ rc_v). }
-          admit.
+          simpl. destruct rc_v; tauto.
         + eapply Hoare_conseq_pre.
           2: { apply (add_go_left_edge_fact3_l _ _ fa). }
-          admit.
+          simpl; tauto. 
         + eapply Hoare_conseq_pre.
-          2: { apply (add_go_left_edge_fact3_l _ _ fa). }
-          admit.
+          2: { apply (add_go_left_edge_fact3_r _ _ fa). }
+          simpl; tauto.
         + eapply Hoare_conseq_pre.
-          2: { apply (add_go_left_edge_fact4_u _ _ lc_fa). }
-          admit. 
-        + eapply Hoare_conseq_pre.
-          2: { apply (add_go_left_edge_fact4_u _ _ rc_fa). }
-          admit.
-      * cbv beta.
+          2: { apply (add_go_left_edge_fact3_u _ _ fa). }
+          simpl; tauto.
+        + assert (Hoare
+                (fun s => BinaryTree.legal s.(heap) /\
+                  (gf = by_empty -> ~ (exists x : Z, BinaryTree.step_u s.(heap) fa x)))
+                (add_go_left_edge' fa rc_fa) 
+                (fun _ s => (dir_fa_v = 0 -> ~ (exists x : Z, BinaryTree.step_u s.(heap) fa x)))).
+      {
+        pose proof remove_go_right_edge'_fact3_u fa rc_fa fa.
+        revert H0.
+        unfold Hoare; sets_unfold; intros.
+        destruct H1.
+        pose proof H4 H3.
+        pose proof H0 _ _ _ H5 H2.
+        tauto.
+
+
+
+      - cbv beta. 
+        apply Hoare_test_bind.
+          eapply Hoare_bind.
+          { 
+            eapply Hoare_conj9.
+            + eapply Hoare_conseq_pre.
+              2: { apply remove_go_right_edge_fact2. }
+              tauto.
+            + eapply Hoare_conseq_pre.
+              2: { apply (remove_go_right_edge_fact3_l _ _ v). }
+              tauto.
+            + eapply Hoare_conseq_pre.
+              2: { apply (remove_go_right_edge_fact3_r _ _ v). }
+              tauto.
+            + eapply Hoare_conseq_pre.
+              2: { apply (remove_go_right_edge_fact4_u _ _ lc_v). }
+              tauto.
+            + eapply Hoare_conseq_pre.
+              2: { apply (remove_go_right_edge_fact4_u _ _ rc_v). }
+              tauto.
+            + eapply Hoare_conseq_pre.
+              2: { apply (remove_go_right_edge_fact3_l _ _ fa). }
+              tauto.
+            + eapply Hoare_conseq_pre.
+              2: { apply (remove_go_right_edge_fact3_r _ _ fa). }
+              tauto.
+            + eapply Hoare_conseq_pre.
+              2: { apply (remove_go_right_edge_fact4_u _ _ lc_fa). }
+              tauto.
+            + eapply Hoare_conseq_pre.
+              2: { apply (remove_go_right_edge_fact4_u _ _ rc_fa). }
+              tauto.  
+          }
+          cbv beta; intros _.
+          eapply Hoare_conj8.
+          + eapply Hoare_conseq_pre.
+            2: { apply add_go_right_edge_fact2. }
+            intros.
+            destruct H0 as [H1 [_ [_ [_ [_ [H2 H3]]]]]].
+            destruct H as [H4 [H5 [H6 _]]].
+            pose proof (classic(dir_fa_v = 0)).
+            destruct H.
+            ++ pose proof H5 H.
+              subst lc_fa.
+              tauto.
+            ++ destruct H4.
+              -- tauto.
+              -- pose proof H6 H0.
+                  subst rc_fa.
+                  tauto.
+          + eapply Hoare_conseq_pre.
+            2: { apply (add_go_right_edge_fact3_l _ _ v). }
+            simpl; tauto.
+          + eapply Hoare_conseq_pre.
+            2: { apply (add_go_right_edge_fact3_r _ _ v). }
+            simpl; tauto.
+          + eapply Hoare_conseq_pre.
+            2: { apply (add_go_right_edge_fact4_u _ _ lc_v). }
+            simpl. destruct lc_v; tauto.
+          + eapply Hoare_conseq_pre.
+            2: { apply (add_go_right_edge_fact4_u _ _ rc_v). }
+            simpl. destruct rc_v; tauto.
+          + eapply Hoare_conseq_pre.
+            2: { apply (add_go_right_edge_fact3_l _ _ fa). }
+            simpl; tauto. 
+          + eapply Hoare_conseq_pre.
+            2: { apply (add_go_right_edge_fact3_r _ _ fa). }
+            simpl; tauto.
+          + eapply Hoare_conseq_pre.
+            2: { apply (add_go_right_edge_fact3_u _ _ fa). }
+            simpl; tauto.
+    * cbv beta.
+      unfold Hoare; sets_unfold; intros.
+      subst s2.
+      tauto.
   }
-    1: {
+  cbv beta; intros _.
+  eapply Hoare_bind.
+  { eapply Hoare_conj6.
+    + eapply Hoare_conseq_pre.
+      2: { apply add_go_left_edge'_fact2. }
+      tauto.
+    + eapply Hoare_conseq_pre.
+      2: { apply (add_go_left_edge'_fact3_l _ _ v). }
+      simpl. tauto.
+    + eapply Hoare_conseq_pre.
+      2: { apply (add_go_left_edge'_fact3_r _ _ v). }
+      simpl; tauto.
+    + eapply Hoare_conseq_pre.
+      2: { apply (add_go_left_edge'_fact4_u _ _ rc_v). }
+      simpl; intros.
+      destruct lc_v.
+      ++ destruct rc_v; tauto.
+      ++ tauto.
+    + eapply Hoare_conseq_pre.
+      2: { apply (add_go_left_edge'_fact3_r _ _ fa). }
+      simpl; tauto.
+    + eapply Hoare_conseq_pre.
+      2: { apply (add_go_left_edge'_fact3_u _ _ fa). }
+      simpl; tauto.
+  }
+  cbv beta; intros _.
+  eapply Hoare_bind.
+  { eapply Hoare_conj4.
+    + eapply Hoare_conseq_pre.
+      2: { apply add_go_right_edge'_fact2. }
+      tauto.
+    + eapply Hoare_conseq_pre.
+      2: { apply (add_go_right_edge'_fact3_l _ _ v). }
+      simpl. tauto.
+    + eapply Hoare_conseq_pre.
+      2: { apply (add_go_right_edge'_fact3_r _ _ v). }
+      simpl; tauto.
+    + eapply Hoare_conseq_pre.
+      2: { apply (add_go_right_edge'_fact3_u _ _ fa). }
+      simpl; tauto.
+  }
+  cbv beta; intros _.
+  eapply Hoare_choice.
+  - apply Hoare_test_bind.
+    apply Hoare_irr_left; intros.
+    eapply Hoare_bind.
+    { eapply Hoare_conj.
+    + eapply Hoare_conseq_pre.
+      2: { apply add_go_left_edge_fact2. }
+      simpl. tauto.
+    + eapply Hoare_conseq_pre.
+      2: { apply (add_go_left_edge_fact4_u _ _ rc_fa). }
+      simpl. intros. destruct rc_fa.
+      ++ tauto. 
+    + eapply Hoare_conseq_pre.
+      2: { apply (add_go_left_edge_fact3_r _ _ v). }
+      simpl; tauto.
+  }
 
-    }
-    
-
-Admitted.
-  (* 
-  - apply (remove_go_left_edge'_fact2 v lc_v). *)
-
-  
-  
-
-
+        
+       
 Fact swap_v_u_helper1: forall (v rc: Z) (V: Z -> Prop),
   Hoare
     (fun s : state =>
